

# Deriving the Least Squares Solution

Supplementary Material for Supervised Learning

Daniel E. Acuna

Associate Professor, University of Colorado Boulder

# Ordinary Least Squares: Mathematical Derivation

In this supplementary material, we will:

- Develop the full mathematical derivation of OLS
- Use calculus to find the parameters that minimize squared error
- Express the solution in matrix form
- Derive the closed-form expressions for optimal parameters

# The Least Squares Problem

We begin with our linear model:

$$\hat{y}_i = \beta_0 + \beta_1 x_i$$

Our goal is to find the values of  $\beta_0$  and  $\beta_1$  that minimize the sum of squared errors:

$$\sum_{i=1}^n (y_i - \hat{y}_i)^2 = \sum_{i=1}^n (y_i - (\beta_0 + \beta_1 x_i))^2$$

# Step 1: Define the Loss Function

We define a loss function  $L(\beta_0, \beta_1)$  representing the sum of squared errors:

$$L(\beta_0, \beta_1) = \sum_{i=1}^n (y_i - (\beta_0 + \beta_1 x_i))^2$$

## Step 2: Find Critical Points by Taking Partial Derivatives

For the optimal values of  $\beta_0$  and  $\beta_1$ , the partial derivatives must equal zero:

$$\frac{\partial L}{\partial \beta_0} = 0 \quad \text{and} \quad \frac{\partial L}{\partial \beta_1} = 0$$

## Step 3: Calculate the Gradients

$$\frac{\partial L}{\partial \beta_0} = -2 \sum_{i=1}^n (y_i - \beta_0 - \beta_1 x_i) = 0$$

$$\frac{\partial L}{\partial \beta_1} = -2 \sum_{i=1}^n (y_i - \beta_0 - \beta_1 x_i) x_i = 0$$

## Step 4: Simplify the Equations

$$\sum_{i=1}^n (y_i - \beta_0 - \beta_1 x_i) = 0$$

$$\sum_{i=1}^n (y_i - \beta_0 - \beta_1 x_i) x_i = 0$$

## Step 5: Rewrite as Normal Equations

Expanding the first equation:

$$\sum_{i=1}^n y_i - \beta_0 \sum_{i=1}^n 1 - \beta_1 \sum_{i=1}^n x_i = 0$$

Which gives us:

$$\beta_0 n + \beta_1 \sum_{i=1}^n x_i = \sum_{i=1}^n y_i$$

Similarly for the second equation:

$$\beta_0 \sum_{i=1}^n x_i + \beta_1 \sum_{i=1}^n x_i^2 = \sum_{i=1}^n x_i y_i$$



## Step 5.5: Matrix Notation for Linear Regression

Let's see how we can represent our regression problem using matrices. First, we define:

- **Design matrix  $\mathbf{X}$ :** A matrix with one row per data point, where the first column is all 1's (for the intercept) and the second column contains the  $x_i$  values
- **Parameter vector  $\beta$ :** Contains the regression coefficients  $[\beta_0, \beta_1]^T$
- **Response vector  $\mathbf{y}$ :** Contains all the observed  $y_i$  values

For example, with  $n$  data points:

$$\mathbf{X} = \begin{bmatrix} 1 & x_1 \\ 1 & x_2 \\ \vdots & \vdots \\ 1 & x_n \end{bmatrix}, \quad \mathbf{y} = \begin{bmatrix} y_1 \\ y_2 \\ \vdots \\ y_n \end{bmatrix}, \quad \boldsymbol{\beta} = \begin{bmatrix} \beta_0 \\ \beta_1 \end{bmatrix}$$

## Step 5.6: Computing $\mathbf{X}^T \mathbf{X}$ - Part 1

Now, let's examine the matrix product  $\mathbf{X}^T \mathbf{X}$ :

$$\mathbf{X}^T \mathbf{X} = \begin{bmatrix} 1 & 1 & \cdots & 1 \\ x_1 & x_2 & \cdots & x_n \end{bmatrix} \begin{bmatrix} 1 & x_1 \\ 1 & x_2 \\ \vdots & \vdots \\ 1 & x_n \end{bmatrix}$$

## Step 5.6: Computing $\mathbf{X}^T \mathbf{X}$ - Part 2

Computing this matrix multiplication:

$$\mathbf{X}^T \mathbf{X} = \begin{bmatrix} \sum_{i=1}^n 1 & \sum_{i=1}^n x_i \\ \sum_{i=1}^n x_i & \sum_{i=1}^n x_i^2 \end{bmatrix} = \begin{bmatrix} n & \sum_{i=1}^n x_i \\ \sum_{i=1}^n x_i & \sum_{i=1}^n x_i^2 \end{bmatrix}$$

## Step 5.7: Computing $\mathbf{X}^T \mathbf{y}$ - Part 1

Similarly, let's compute  $\mathbf{X}^T \mathbf{y}$ :

$$\mathbf{X}^T \mathbf{y} = \begin{bmatrix} 1 & 1 & \cdots & 1 \\ x_1 & x_2 & \cdots & x_n \end{bmatrix} \begin{bmatrix} y_1 \\ y_2 \\ \vdots \\ y_n \end{bmatrix}$$

## Step 5.7: Computing $\mathbf{X}^T \mathbf{y}$ - Part 2

This gives us:

$$\mathbf{X}^T \mathbf{y} = \begin{bmatrix} \sum_{i=1}^n y_i \\ \sum_{i=1}^n x_i y_i \end{bmatrix}$$

# Step 5.8: Matrix Form of the Normal Equations - Part 1

Recall our normal equations:

$$\beta_0 n + \beta_1 \sum_{i=1}^n x_i = \sum_{i=1}^n y_i$$

$$\beta_0 \sum_{i=1}^n x_i + \beta_1 \sum_{i=1}^n x_i^2 = \sum_{i=1}^n x_i y_i$$

We can write these in matrix form as:

$$\begin{bmatrix} n & \sum_{i=1}^n x_i \\ \sum_{i=1}^n x_i & \sum_{i=1}^n x_i^2 \end{bmatrix} \begin{bmatrix} \beta_0 \\ \beta_1 \end{bmatrix} = \begin{bmatrix} \sum_{i=1}^n y_i \\ \sum_{i=1}^n x_i y_i \end{bmatrix}$$

# Step 5.8: Matrix Form of the Normal Equations - Part 2

Which is precisely:

$$\mathbf{X}^T \mathbf{X} \boldsymbol{\beta} = \mathbf{X}^T \mathbf{y}$$



## Step 6: Express in Matrix Form

We can write this system as  $\mathbf{X}^T \mathbf{X} \boldsymbol{\beta} = \mathbf{X}^T \mathbf{y}$ , where:

- $\mathbf{X}$  is the design matrix with first column of 1s and second column of  $x_i$  values
- $\boldsymbol{\beta} = [\beta_0, \beta_1]^T$  is the parameter vector
- $\mathbf{y} = [y_1, y_2, \dots, y_n]^T$  is the vector of observed outputs

For example, with 3 data points:

$$\mathbf{X} = \begin{bmatrix} 1 & x_1 \\ 1 & x_2 \\ 1 & x_3 \end{bmatrix}, \quad \mathbf{y} = \begin{bmatrix} y_1 \\ y_2 \\ y_3 \end{bmatrix}, \quad \boldsymbol{\beta} = \begin{bmatrix} \beta_0 \\ \beta_1 \end{bmatrix}$$

## Step 7: Solve for the Parameters

Multiplying both sides by  $(\mathbf{X}^T \mathbf{X})^{-1}$  :

$$\beta = (\mathbf{X}^T \mathbf{X})^{-1} \mathbf{X}^T \mathbf{y}$$

For simple linear regression, this gives us:

$$\beta_1 = \frac{\sum_{i=1}^n (x_i - \bar{x})(y_i - \bar{y})}{\sum_{i=1}^n (x_i - \bar{x})^2} = \frac{Cov(X, Y)}{Var(X)}$$

$$\beta_0 = \bar{y} - \beta_1 \bar{x}$$

Where  $\bar{x}$  and  $\bar{y}$  are the means of  $x$  and  $y$  values respectively.

# Geometric Interpretation

The least squares solution has an important geometric interpretation:

- The residuals are orthogonal (perpendicular) to the column space of  $\mathbf{X}$
- The predicted values  $\hat{\mathbf{y}}$  are the orthogonal projection of  $\mathbf{y}$  onto the column space of  $\mathbf{X}$
- This is the closest point in the column space to the actual  $\mathbf{y}$

# Example: Calculating OLS Parameters

Consider this small dataset:

x	y
1	2
2	3
3	5

Let's calculate: -  $\bar{x} = \frac{1+2+3}{3} = 2$  -  $\bar{y} = \frac{2+3+5}{3} = \frac{10}{3} \approx 3.33$  -

$$\sum (x_i - \bar{x})(y_i - \bar{y}) = (1 - 2)(2 - 3.33) + (2 - 2)(3 - 3.33) + (3 - 2)(5 - 3.33) = 2.67$$

$$- \sum (x_i - \bar{x})^2 = (1 - 2)^2 + (2 - 2)^2 + (3 - 2)^2 = 2$$

$$\text{Therefore: - } \beta_1 = \frac{2.67}{2} = 1.33 \text{ - } \beta_0 = 3.33 - 1.33 \times 2 = 0.67$$

Our fitted line is:  $\hat{y} = 0.67 + 1.33x$

# Summary: The Least Squares Method

Key points about the OLS derivation:

- We use calculus to find parameter values that minimize squared error
- The solution involves setting partial derivatives to zero
- The normal equations can be solved using matrix algebra
- The closed-form solution is  $\beta = (\mathbf{X}^T \mathbf{X})^{-1} \mathbf{X}^T \mathbf{y}$
- For simple linear regression, parameters depend on means and covariances
- This approach generalizes to multiple regression with many predictors